deps/poulet4/lib/Monads/Monad.v
@@ -53,6 +53,19 @@ Definition lift_monad {A B} {m: Type -> Type} {M : Monad m} (f: A -> B) (ma : m 
 
 Notation "c '>>|' f" := (lift_monad f c) (at level 50, left associativity) : monad_scope.
 
+Lemma map_bind_pair :
+  forall (M : Type -> Type) `{MM: Monad M}
+    (T U V W : Type) (f : T -> V) (g : U -> M W) tus,
+    List.map (fun '(t,u) => g u >>| pair (f t)) tus =
+    List.map
+      (fun '(v,ow) => ow >>| @pair V W v)
+      (combine (map f (map fst tus)) (map g (map snd tus))).
+Proof.
+  intros M MM T U V W f g tus.
+  induction tus as [| [t u] tus IHtus];
+    cbn in *; f_equal; auto.
+Qed.
+
 Notation "x '<<|' c1 ;; c2" := (lift_monad (fun x => c2) c1)
   ( at level 100, c1 at next level,
     format "x  '<<|'  c1 ';;' '//' c2",
